KLR/KLR/Operators.lean
@@ -1,12 +1,72 @@
 /-
 Copyright (c) 2025 Amazon.com, Inc. or its affiliates. All Rights Reserved.
 Released under Apache 2.0 license as described in the file LICENSE.
-Authors: Paul Govereau, Sean McLaughlin
+Authors: Paul Biberstein, Pavel Potapov, Markus De Medeiros
 -/
 
 import KLR.KLR.Basic
 
 namespace KLR.KLR
+
+/-
+ALU operations supported by the HW
+Only used by: TensorScalar, TensorScalarPtr, TensorReduce, TensorTensor
+-/
+
+inductive AluOp where
+  | abs
+  | add
+  | arith_shift_left
+  | arith_shift_right
+  | average
+  | bitwise_and
+  | bitwise_not
+  | bitwise_or
+  | bitwise_xor
+  | bypass
+  | divide
+  | is_equal
+  | is_ge
+  | is_gt
+  | is_le
+  | is_lt
+  | logical_and
+  | logical_or
+  | logical_shift_left
+  | logical_shift_right
+  | logical_xor
+  | max
+  | min
+  | mod
+  | mult
+  | not_equal
+  | pow
+  | rsqrt
+  | subtract
+  deriving BEq, Repr
+
+namespace AluOp
+
+def isBitwise : AluOp -> Bool
+  | arith_shift_left
+  | arith_shift_right
+  | bitwise_not
+  | bitwise_and
+  | bitwise_or
+  | bitwise_xor
+  | logical_shift_left
+  | logical_shift_right
+  | bypass => true
+  | _ => false
+
+def isArith : AluOp -> Bool
+  | .bypass => true
+  | op => not op.isBitwise
+
+instance : ToString AluOp where
+  toString op := reprStr op
+
+end AluOp
 
 inductive DropoutThresholdType
   | DropRate
@@ -93,8 +153,8 @@ def AluOp.IsTensorReduceBitwiseOp  : AluOp → Prop
 
 
 structure Dropout where
-  dst           : TensorView
-  src           : TensorView
+  dst           : TensorRef
+  src           : TensorRef
   thresholdType : DropoutThresholdType
   threshold     : Immediate
 
@@ -102,8 +162,8 @@ structure Dropout where
 `OUT accum= activate_func( (IN * scale_value)] + bias, imm )`
 -/
 structure Activate where
-  dst             : TensorView
-  src             : TensorView
+  dst             : TensorRef
+  src             : TensorRef
   accumulatorCmd  : AccumCmd
   activationFunc  : ActivationFunc
   scale           : Immediate
@@ -116,8 +176,8 @@ the comparison is true, the value from `in` is used, otherwise `fill_value` is u
 out[k] = (mask[k] <op> 0) ? in[k]  : fill_value
 -/
 structure AffineSelect where
-  dst         : TensorView
-  src         : TensorView
+  dst         : TensorRef
+  src         : TensorRef
   fillMode    : AffineSelectCmp
   fillReg     : Reg
   maskPattern : DataPattern
@@ -129,8 +189,8 @@ TODO: this operation is stateful since it uses the DMA queues. How
 do we represent that at the KLR level?
 -/
 structure DmaCopy where
-  dst            : TensorView
-  src            : TensorView
+  dst            : TensorRef
+  src            : TensorRef
   compute_op     : DgeComputeOp
   dstBoundsCheck : DMABounds
   srcBoundsCheck : DMABounds
@@ -139,8 +199,8 @@ structure DmaCopy where
 Use the DMA to reverse the dimensions of a tensor.
 -/
 structure DmaTranspose where
-  dst : TensorView
-  src : TensorView
+  dst : TensorRef
+  src : TensorRef
 
 /-
 Uses the DVE engine to do a transpose on 32x32 tiles of tensors up to 4d.
@@ -150,8 +210,8 @@ must be the same size. The number of partitions must be a multiple of 32.
 OR use the PE engine to do a transpose on 2d tensors, where the normal PE engine restrictions apply.
 -/
 structure Transpose where
-  dst : TensorView
-  src : TensorView
+  dst : TensorRef
+  src : TensorRef
   engine : Engine
 
 /-
@@ -166,43 +226,43 @@ structure LoadMaskRegister where
 Use the DVE to shuffle the data in src into dst based on MaskRegister
 -/
 structure Shuffle where
-  dst : TensorView
-  src : TensorView
+  dst : TensorRef
+  src : TensorRef
   --shuffle_pattern : Reg
 
 /- Sets `count` elements of `dst` to `value` -/
 structure MemSet where
-  dst   : TensorView
+  dst   : TensorRef
   value : UInt32
   count : Nat
 
 /- Generates values using `src` and writes them to `dst` -/
 structure Iota where
-  dst : TensorView
+  dst : TensorRef
   src : DataPattern
 
 /- Loads a matrix into the PE -/
 structure LoadStationary where
-  src         : TensorView
+  src         : TensorRef
   isTranspose : Bool
 
 /- Performs a matmul using the PE -/
 structure MatMul where
-  dst                : TensorView
-  moving             : TensorView
+  dst                : TensorRef
+  moving             : TensorRef
   psumAccumulateFlag : MatmulGroupElement
 
 structure LocalGather where
-  dst               : TensorView
-  src               : TensorView
+  dst               : TensorRef
+  src               : TensorRef
   indexMissBehavior : IndexMissBehavior
   /- Set to true when this is the last local gather operation in a group
   to free the pool buffer -/
   freePoolBuffer    : Bool
 
 structure RangeSelect where
-  dst            : TensorView
-  src            : TensorView
+  dst            : TensorRef
+  src            : TensorRef
   reduceCommand  : AccumCmd
   reduceOp       : AluOp
   base           : Float32
@@ -223,9 +283,9 @@ if (accumulator_cmd == ZeroAccumulator) or (accumulator_cmd == Accumulator):
 ```
 -/
 structure ScalarTensorTensor where
-  dst             : TensorView
-  src0            : TensorView
-  src1            : TensorView
+  dst             : TensorRef
+  src0            : TensorRef
+  src1            : TensorRef
   op0             : AluOp
   op1             : AluOp
   reverseOperands : TensorScalarReverseOps
@@ -234,9 +294,9 @@ structure ScalarTensorTensor where
 
 /- Copies each element from src to dst for which predicate is not 0 -/
 structure CopyPredicated where
-  dst       : TensorView
-  src       : TensorView
-  predicate : TensorView
+  dst       : TensorRef
+  src       : TensorRef
+  predicate : TensorRef
 
 /-
 for lane_id in range(num_active_channels):
@@ -247,9 +307,9 @@ for lane_id in range(num_active_channels):
         dst_mem_pattern.append(new_result)
 -/
 structure TensorTensorScan where
-  dst             : TensorView
-  src0            : TensorView
-  src1            : TensorView
+  dst             : TensorRef
+  src0            : TensorRef
+  src1            : TensorRef
   op0             : AluOp
   op1             : AluOp
   reverseOperands : TensorScalarReverseOps
@@ -258,91 +318,110 @@ structure TensorTensorScan where
 
 /- Loads values into the DVE's MatchValue registers -/
 structure MatchValueLoad where
-  src : TensorView
+  src : TensorRef
 
 /- For each element in MatchValue register, find the first element of src that
 matches and stores its index in dst. -/
 structure FindIndex8 where
-  dst : TensorView
-  src : TensorView
+  dst : TensorRef
+  src : TensorRef
 
 /- Same as FindIndex8, but replaces the found values in src with `replaceValue`-/
 structure MatchReplace8 where
-  dst          : TensorView
-  src          : TensorView
+  dst          : TensorRef
+  src          : TensorRef
   replaceValue : Float32
 
 /- Finds the 8 largest values in src and writes them to dst -/
 structure Max8 where
-  dst : TensorView
-  src : TensorView
+  dst : TensorRef
+  src : TensorRef
 
 -- TODO : @govereau do we need to support these custom ops if they're Sunda-specific?
+/-
 inductive SundaAddr
-
 inductive CustomOpArgLocation where
 | Invalid
 | Sbuf
 | Hbm
-
 abbrev TPBAddr  := UInt32
-
 inductive CustomOpTensorShape where
 | InlineShape8d (data : List UInt16) -- there are 8 of these
 | OutOfLineShape (addr : TPBAddr)
 | InlineShape4d (data : List UInt32) -- there are 4 of these
-
 inductive CustomOpTensorStorage where
 | tpb (addr : TPBAddr) (num_elem : UInt32) (num_partitions : UInt8) (num_elemens_per_block : UInt32)
 | hbm (addr : SundaAddr) (num_elem : UInt32)
-
 structure CustomOpArgTensor where
   location        : CustomOpArgLocation
   framework_shape : CustomOpTensorShape
   storage         : CustomOpTensorStorage
-
 structure CustomOpArgArrayOfTensor where
   num_object : UInt32
-
 inductive CustomOpArgType where
 | Invalid
 | Tensor
 | ArrayOfTensor
-
 inductive CustomOpArgUnion where
 | tensor (t : CustomOpArgTensor)
 | array_of_tensor (ar : CustomOpArgArrayOfTensor)
-
 structure CustomOpPayload where
   arg : CustomOpArgUnion
+-/
 
 structure BatchNormAggregate where
-  dst : TensorView
-  src : TensorView
+  dst : TensorRef
+  src : TensorRef
 
 structure BatchNormStats where
-  dst : TensorView
-  src : TensorView
+  dst : TensorRef
+  src : TensorRef
 
 structure Reciprocal where
-  dst  : TensorView
-  src  : TensorView
+  dst  : TensorRef
+  src  : TensorRef
 
 /- Copy src to dst -/
 structure Copy where
-  dst   : TensorView
-  src   : TensorView
+  dst   : TensorRef
+  src   : TensorRef
   /- TODO: what is this for? -/
   opDim : Option TensorSubDim
   --copy_dim  : op_dim.IsCopySubDim
 
 /- Reduces a tensor along specified dimensions -/
 structure TensorReduce where
-  dst          : TensorView
-  src          : TensorView
+  dst          : TensorRef
+  src          : TensorRef
   op           : AluOp
   opDim        : TensorSubDim
   -- the negated field is only relevant for arithmetic operations
   negated      : Bool
 
-inductive Operator
+inductive Operator where
+  | Activate (op : Activate)
+  | AffineSelect (op : AffineSelect)
+  | BatchNormAggregate (op : BatchNormAggregate)
+  | BatchNormStats (op : BatchNormStats)
+  | Copy (op : Copy)
+  | CopyPredicated (op : CopyPredicated)
+  | DmaCopy (op : DmaCopy)
+  | DmaTranspose (op : DmaTranspose)
+  | Dropout (op : Dropout)
+  | FindIndex8 (op : FindIndex8)
+  | Iota (op : Iota)
+  | LoadMaskRegister (op : LoadMaskRegister)
+  | LoadStationary (op : LoadStationary)
+  | LocalGather (op : LocalGather)
+  | MatMul (op : MatMul)
+  | MatchReplace8 (op : MatchReplace8)
+  | MatchValueLoad (op : MatchValueLoad)
+  | Max8 (op : Max8)
+  | MemSet (op : MemSet)
+  | RangeSelect (op : RangeSelect)
+  | Reciprocal (op : Reciprocal)
+  | ScalarTensorTensor (op : ScalarTensorTensor)
+  | Shuffle (op : Shuffle)
+  | TensorReduce (op : TensorReduce)
+  | TensorTensorScan (op : TensorTensorScan)
+  | Transpose (op : Transpose)
